Prove [disk_size_ok']. Much room for cleanup.

src/ReplicatedDisk/ReplicatedDiskImpl.v
@@ -917,47 +917,53 @@ Module ReplicatedDisk.
 
     Definition td_disk_size_post (state:TD.State) v :=
       match (TD.get_disk d0 state, TD.get_disk d1 state) with
-      | (Some d', Some d'') => d' = d'' /\ size d' = v /\ size d'' = v
+      | (Some d', Some d'') => size d' = v /\ size d'' = v
       | (Some d', None) => size d' = v
       | (None, Some d'') => size d'' = v
       | (None, None) => False
       end.
 
-    Lemma td_disk_size_ok': forall (state:TD.State) id v,
-      td_disk_size_pre state ->
-      disk_size state id v ->
-      td_disk_size_post state v.
+    Lemma recovery_pre_failure: forall state state' s,
+      recovery_pre state s ->
+      TD.bg_failure state state' ->
+      recovery_pre state' s.
     Proof.
-      intros. 
-      unfold disk_size, td_disk_size_pre, td_disk_size_post in *.
-      destruct state; simpl in *.
-      destruct disk0; simpl in *.
-      destruct disk1; simpl in *.
-      - intuition; subst.
-        + destruct id; simpl in *.
-          inversion H0; auto.
-          inversion H0; auto.
-        + destruct id; simpl in *.
-          inversion H0; auto.
-          inversion H0; auto.
-      - destruct id; simpl in *.
-        inversion H0; try congruence.
-        inversion H0; try congruence.
-      - destruct disk1; simpl in *.
-        + destruct id; simpl in *.
-          inversion H0; auto.
-          inversion H0; auto.
-        + destruct some_disk_works; auto.
+      intros.
+      TD.inv_bg.
+      + auto.
+      + unfold recovery_pre in *; simpl in *.
+        intuition.
+        repeat deex.
+        intuition.
+        right. exists a, b. split; auto.
+      + unfold recovery_pre in *; simpl in *.
+        intuition.
+        repeat deex.
+        intuition.
+        - right. exists a, b. split; auto.
+        - right. exists a, b. split; auto.
     Qed.
 
-    (* disk size without recovery *)
-    Lemma disk_size_ok': forall v w w' state,
+    Lemma bg_failure_disk: forall id (state:TD.State) state',
+      TD.get_disk id state = None ->
+      TD.bg_failure state state' ->
+      TD.get_disk id state' = None.
+    Proof.
+      intros.
+      TD.inv_bg.
+      - eauto.
+      - destruct id; simpl in *; eauto.
+      - destruct id; simpl in *; eauto.
+    Qed.
+
+    (* disk size on post-crash, pre-recovery state *)
+    Lemma disk_size_ok': forall v w w' state s,
       abstraction (interface_abs td) w state ->
-      td_disk_size_pre state ->
+      recovery_pre state s ->
       exec diskSize w (Finished v w') ->
       exists state',
         abstraction (interface_abs td) w' state' /\
-        td_disk_size_post state' v.
+        td_disk_size_post state' v /\ recovery_pre state' s.
     Proof.
       intros.
       inv_exec.
@@ -965,37 +971,80 @@ Module ReplicatedDisk.
       - eapply RExec in H7.
         eapply impl_ok in H7; eauto. deex.
         exec_steps; repeat ( ReplicatedDisk.inv_bg || ReplicatedDisk.inv_step ).
-        TD.inv_step.
-        + eapply td_disk_size_ok' in H6.
-          eexists. split; eauto.
-          admit.
-        + simpl; auto. 
-      - eapply RExec in H7.
-        eapply impl_ok in H7; eauto. deex.
-        eapply RExec in H9.
-        inv_rexec.
+        TD.inv_step; simpl in *.
+        + eapply recovery_pre_failure in H2; eauto. 
+          exists state'.
+          split; auto.
+          split; auto.
+          case_eq (TD.disk0 state'); intros.
+          -- rewrite H3 in H6; simpl in *.
+            inversion H6.
+            unfold td_disk_size_post.
+            unfold recovery_pre in H2; simpl in *.
+            rewrite H3 in *; simpl in *.
+            case_eq (TD.disk1 state'); intros; auto.
+            ++  rewrite H4 in *; simpl in *.
+              intuition; subst; auto.
+              repeat deex.
+              intuition; subst; auto.
+              rewrite diskUpd_size; auto.
+          -- rewrite H3 in H6; simpl in *.
+            inversion H6; auto.
+        + simpl; auto.
+      - 
         inv_exec.
         destruct v0.
-        + eapply RExec in H9.
-          eapply impl_ok in H9; eauto. deex.
+        + inv_exec.
+          eapply RExec in H7.
+          eapply impl_ok in H7; eauto. deex.
+          eapply RExec in H6.
+          eapply impl_ok in H6; eauto. deex.
           exec_steps; repeat ( ReplicatedDisk.inv_bg || ReplicatedDisk.inv_step ).
           TD.inv_step.
-          eapply td_disk_size_ok' in H9.
-          eexists. split; eauto.
-          admit.
-          simpl; auto.
-        + eapply RExec in H9.
-          eapply impl_ok in H9; eauto. deex.
+          TD.inv_step.
+          simpl in *.
+          case_eq (TD.disk0 state'); intros.
+          -- rewrite H5 in H8. inversion H8.
+          -- rewrite H5 in H8.
+             case_eq (TD.disk1 state'0); intros.
+             ++ rewrite H6 in H9.
+              inversion H9.
+              eapply bg_failure_disk with (id := d0) in H5 as H5'; eauto.
+              exists state'0.
+              split; auto.
+              eapply recovery_pre_failure in H2; eauto.
+              eapply recovery_pre_failure in H4; eauto.
+              split; auto.
+              unfold td_disk_size_post. subst; simpl.
+              rewrite H6; simpl in *.
+              rewrite H5'; simpl; auto.
+            ++ 
+              eapply bg_failure_disk with (id := d0) in H4 as H4'; simpl in *.
+              apply both_disks_not_missing in H6; eauto.
+              exfalso; auto. auto.
+         -- simpl; auto.
+         -- simpl; auto.
+        + inv_exec.
+          eapply RExec in H7.
+          eapply impl_ok in H7; eauto. deex.
+          eapply RExec in H6.
+          eapply impl_ok in H6; eauto. deex.
           exec_steps; repeat ( ReplicatedDisk.inv_bg || ReplicatedDisk.inv_step ).
-          eexists. split; eauto.
-          eapply td_disk_size_none_ok in H6 as H6; eauto.
-          admit.
-          simpl; auto.
-        + simpl; auto.
+          TD.inv_step.
+          TD.inv_step.
+          simpl in *.
+          case_eq (TD.disk1 state'0); intros; rewrite H5 in *.
+          -- inversion H9.
+          -- case_eq (TD.disk0 state'); intros; rewrite H6 in *.
+             ++ inversion H8.
+             ++ eapply bg_failure_disk with (id := d0) in H4 as H4'; simpl in *; auto.
+              apply both_disks_not_missing in H5; eauto.
+              exfalso; auto.
+          -- simpl; auto.
+          -- simpl; auto.
       Unshelve.
-      all: eauto; try exact unit. 
-      constructor.
-    Admitted.
+      all: eauto; try exact unit.
+    Qed.
 
     Lemma recover_finish_ok: forall w w' s state,
       abstraction (interface_abs td) w state ->
